Freigen/CompM/Examples/Nondet/Defs.lean
@@ -6,18 +6,15 @@ namespace Freigen.CompM.Examples.Nondet
 
 inductive Eff : Type
 | rand
-| print
+| print (z : ℤ)
 
 abbrev Effects : Unit → Type := fun _ => Eff
 abbrev Stack := Eff.Tau ⊕ₑ Effects
 
 instance : Eff.Spec Effects where
-  input
-    | _, .rand => Unit
-    | _, .print => ℤ
   output
     | _, .rand => ℤ
-    | _, .print => Unit
+    | _, .print _ => Unit
   blockTag := fun _ _ => Empty
   blockCtx := nofun
   blockInputs := nofun
@@ -30,10 +27,10 @@ abbrev Nondet α := CompM Nondet.Stack () α
 namespace Nondet
 
 def rand : Nondet ℤ :=
-  CompM.op (E := Stack) (Sum.inr Eff.rand) () nofun
+  CompM.op (E := Stack) (Sum.inr Eff.rand) nofun
 
 def print (z : ℤ) : Nondet Unit :=
-  CompM.op (E := Stack) (Sum.inr Eff.print) z nofun
+  CompM.op (E := Stack) (Sum.inr (Eff.print z)) nofun
 
 def approxWith {α} (entropy : ℕ → ℤ) (t : Nondet α) (n: Nat): List ℤ :=
   go (entropy, 0) n ((t.run pure).approx n) where
@@ -43,8 +40,8 @@ def approxWith {α} (entropy : ℕ → ℤ) (t : Nondet α) (n: Nat): List ℤ :
    | 0, IxPoly.M.Approx.zero _ => []
    | n+1, IxPoly.M.Approx._succ _ _ p k => match p with
      | .ret _ => []
-     | .op (Sum.inr Eff.rand) () => go (entropy.1, entropy.2 + 1) n (k $ .inl (entropy.1 entropy.2))
-     | .op (Sum.inr Eff.print) z => z :: go entropy n (k $ .inl ())
-     | .op (Sum.inl _) _ => go entropy n (k $ .inl ())
+     | .op (Sum.inr Eff.rand) => go (entropy.1, entropy.2 + 1) n (k $ .inl (entropy.1 entropy.2))
+     | .op (Sum.inr (Eff.print z)) => z :: go entropy n (k $ .inl ())
+     | .op (Sum.inl _) => go entropy n (k $ .inl ())
 
 end Freigen.CompM.Examples.Nondet
